src/Lean/Elab/Do.lean
@@ -588,7 +588,10 @@ else
 namespace ToTerm
 
 inductive Kind
-| regular | forInNestedTerm | forIn | forInMap
+| regular
+| forInNestedTerm
+| forIn
+| forInMap (x : Name)
 
 structure Context :=
 (m     : Syntax) -- Syntax to reference the monad associated with the do notation.
@@ -614,12 +617,22 @@ else do
   uvars ← mkUVarTuple ref;
   liftM $ mkTuple ref #[val, uvars]
 
+private def mkForInYield (ref : Syntax) : M Syntax := do
+u ← mkUVarTuple ref;
+`(HasPure.pure (ForInStep.yield $u))
+
+private def mkForInMapYield (ref : Syntax) (x : Name) : M Syntax := do
+u ← mkUVarTuple ref;
+r ← liftM $ mkTuple ref #[mkIdentFrom ref x, u];
+`(HasPure.pure (ForInStep.yield $r))
+
 def returnToTermCore (ref : Syntax) (val : Syntax) : M Syntax := do
 ctx ← read;
 match ctx.kind with
 | Kind.forInNestedTerm => do u ← mkUVarTuple ref; `(HasPure.pure (DoResult.«return» $u))
 | Kind.regular         => do r ← mkResultUVarTuple ref val; `(HasPure.pure $r)
-| _                    => do u ← mkUVarTuple ref; `(HasPure.pure (ForInStep.yield $u))
+| Kind.forIn           => mkForInYield ref
+| Kind.forInMap x      => mkForInMapYield ref x
 
 def returnToTerm (ref : Syntax) (val : Syntax) : M Syntax := do
 r ← returnToTermCore ref val;
@@ -630,7 +643,8 @@ ctx ← read;
 match ctx.kind with
 | Kind.regular         => unreachable!
 | Kind.forInNestedTerm => do u ← mkUVarTuple ref; `(HasPure.pure (DoResult.«continue» $u))
-| _                    => do u ← mkUVarTuple ref; `(HasPure.pure (ForInStep.yield $u))
+| Kind.forIn           => mkForInYield ref
+| Kind.forInMap x      => mkForInMapYield ref x
 
 def continueToTerm (ref : Syntax) : M Syntax := do
 r ← continueToTermCore ref;
@@ -641,7 +655,8 @@ ctx ← read;
 match ctx.kind with
 | Kind.regular         => unreachable!
 | Kind.forInNestedTerm => do u ← mkUVarTuple ref; `(HasPure.pure (DoResult.«break» $u))
-| _                    => do u ← mkUVarTuple ref; `(HasPure.pure (ForInStep.done $u))
+| Kind.forIn           => do u ← mkUVarTuple ref; `(HasPure.pure (ForInStep.done $u))
+| Kind.forInMap x      => do u ← mkUVarTuple ref; r ← liftM $ mkTuple ref #[mkIdentFrom ref x, u]; `(HasPure.pure (ForInStep.done $r))
 
 def breakToTerm (ref : Syntax) : M Syntax := do
 r ← breakToTermCore ref;
@@ -748,25 +763,9 @@ partial def toTerm : Code → M Syntax
 | Code.ite ref _ o c t e  => do t ← toTerm t; e ← toTerm e; pure $ mkIte ref o c t e
 | _ => liftM $ Macro.throwError Syntax.missing "WIP"
 
-private def getKindUVars (c : CodeBlock) (forInVar? : Option Name) : Kind × Array Name :=
-match forInVar? with
-| none          =>
-  if hasContinueBreak c.code then
-    (Kind.forInNestedTerm, nameSetToArray c.uvars)
-  else
-    (Kind.regular, nameSetToArray c.uvars)
-| some forInVar =>
-  if c.uvars.contains forInVar then
-    let uvars := #[forInVar] ++ nameSetToArray (c.uvars.erase forInVar);
-    (Kind.forInMap, uvars)
-  else
-    (Kind.forIn, nameSetToArray c.uvars)
-
-def run (c : CodeBlock) (m : Syntax) (forInVar? : Option Name := none) : MacroM (Array Name × Syntax) := do
-let code := c.code;
-let (kind, uvars) := getKindUVars c forInVar?;
+def run (code : Code) (m : Syntax) (uvars : Array Name := #[]) (kind := Kind.regular) : MacroM Syntax := do
 term ← toTerm code { m := m, kind := kind, uvars := uvars };
-pure (uvars, term)
+pure term
 
 end ToTerm
 
@@ -778,6 +777,27 @@ structure Context :=
 (insideFor : Bool := false)
 
 abbrev M := ReaderT Context TermElabM
+
+@[inline] def withFor {α} (x : M α) : M α :=
+adaptReader (fun (ctx : Context) => { ctx with insideFor := true }) x
+
+structure ToForInTermResult :=
+(isForInMap : Bool)
+(uvars      : Array Name)
+(term       : Syntax)
+
+def toForInTerm  (x : Syntax) (forCodeBlock : CodeBlock) : M ToForInTermResult := do
+ctx ← read;
+let uvars := forCodeBlock.uvars;
+if x.isIdent && uvars.contains x.getId then do
+  -- It is a forInMap
+  let uvars := nameSetToArray (uvars.erase x.getId);
+  term ← liftMacroM $ ToTerm.run forCodeBlock.code ctx.m uvars (ToTerm.Kind.forInMap x.getId);
+  pure ⟨true, uvars, term⟩
+else do
+  let uvars := nameSetToArray uvars;
+  term ← liftMacroM $ ToTerm.run forCodeBlock.code ctx.m uvars ToTerm.Kind.forIn;
+  pure ⟨false, uvars, term⟩
 
 def ensureInsideFor : M Unit := do
 ctx ← read;
@@ -869,8 +889,23 @@ partial def doSeqToCode : List Syntax → M CodeBlock
       body ← doSeqToCode (getDoSeqElems doSeq);
       unless ← liftM $ mkUnless ref cond body;
       concatWithRest unless
-    else if k == `Lean.Parser.Term.doFor then
-      throwError "WIP"
+    else if k == `Lean.Parser.Term.doFor then withFreshMacroScope do
+      let ref       := doElem;
+      let x         := doElem.getArg 1;
+      let xs        := doElem.getArg 3;
+      let forElems  := getDoSeqElems (doElem.getArg 5);
+      forCodeBlock  ← withFor (doSeqToCode forElems);
+      ⟨isForInMap, uvars, forInBody⟩ ← toForInTerm x forCodeBlock;
+      uvarsTuple ← liftMacroM $ mkTuple ref (uvars.map (mkIdentFrom ref));
+      auxDo ← if isForInMap then do
+        forInTerm ← `($(xs).forInMap $uvarsTuple fun $x $uvarsTuple => $forInBody);
+        `(do let r ← $forInTerm; $uvarsTuple:term := r.2; return r.1)
+      else do {
+        forInTerm ← `($(xs).forIn $uvarsTuple fun $x $uvarsTuple => $forInBody);
+        `(do let r ← $forInTerm; $uvarsTuple:term := r)
+      };
+      let doElemsNew := getDoSeqElems (getDoSeq auxDo);
+      doSeqToCode (doElemsNew ++ doElems)
     else if k == `Lean.Parser.Term.doMatch then
       throwError "WIP"
     else if k == `Lean.Parser.Term.doTry then
@@ -927,7 +962,7 @@ fun stx expectedType? => do
   m ← mkMonadAlias bindInfo.m;
   codeBlock ← ToCodeBlock.run stx m;
   -- trace! `Elab.do ("codeBlock: " ++ Format.line ++ codeBlock.toMessageData);
-  (_, stxNew) ← liftMacroM $ ToTerm.run { codeBlock with uvars := {} }  m;
+  stxNew ← liftMacroM $ ToTerm.run codeBlock.code m;
   trace! `Elab.do stxNew;
   let expectedType := mkApp bindInfo.m bindInfo.α;
   withMacroExpansion stx stxNew $ elabTermEnsuringType stxNew expectedType
